Prove all subgoals for nondeterministic version, leaving alloc lemma and Qed to do

src/Bedrock/Group/ScalarMult/LadderStep.v
@@ -5,6 +5,13 @@ Require Import Crypto.Bedrock.Group.Point.
 Require Import Crypto.Bedrock.Specs.Field.
 Local Open Scope Z_scope.
 
+(*TODO: currently relies on Examples files.
+  This file should either be moved somewhere else or the dependency removed.
+*)
+Require Import Rupicola.Examples.Nondeterminism.NonDeterminism.
+Require Import Rupicola.Examples.Nondeterminism.StackAlloc.
+Import NDMonad.
+
 Section __.
   Context {width: Z} {BW: Bitwidth width} {word: word.word width} {mem: map.map word Byte.byte}.
   Context {locals: map.map String.string word}.
@@ -19,11 +26,51 @@ Section __.
           {field_representation_ok : FieldRepresentation_ok}.
   Hint Resolve relax_bounds : compiler.
 
+  (*Modified from stack_alloc*)
+  Definition felem_alloc : Comp (felem) := fun _ => True.
+
+  Lemma compile_stack_alloc {tr mem locals functions}:
+    let c := felem_alloc in
+    forall {B} {pred: B -> predicate}
+      {k: felem -> Comp B} {k_impl}
+      (R: _ -> Prop) var,
+      R mem ->
+      (forall ptr (bs: felem) mem,
+          (FElem ptr bs * R)%sep mem ->
+          let pred g tr' mem' locals' :=
+              exists R' bs',
+                (FElem ptr bs' * R')%sep mem' /\
+                forall mem'', R' mem'' -> pred g tr' mem'' locals' in
+          <{ Trace := tr;
+             Memory := mem;
+             Locals := map.put locals var ptr;
+             Functions := functions }>
+          k_impl
+          <{ pbind pred (k bs) }>) ->
+      <{ Trace := tr;
+         Memory := mem;
+         Locals := locals;
+         Functions := functions }>
+      cmd.stackalloc var felem_size_in_bytes k_impl
+      <{ pbind pred (bindn [var] c k) }>.
+  Proof.
+  Admitted.
+
+
   Section Gallina.
     Local Open Scope F_scope.
 
     Definition ladderstep_gallina
-               (X1: F M_pos) (P1 P2: point)  : (point * point) :=
+               (X1: F M_pos) (P1 P2: point) : Comp (point * point) :=
+      let/+ A := felem_alloc in
+      let/+ AA := felem_alloc in
+      let/+ B := felem_alloc in
+      let/+ BB := felem_alloc in
+      let/+ E := felem_alloc in
+      let/+ C := felem_alloc in
+      let/+ D := felem_alloc in
+      let/+ DA := felem_alloc in
+      let/+ CB := felem_alloc in
       let '(X2, Z2) := P1 in
       let '(X3, Z3) := P2 in
       let/n A := X2+Z2 in
@@ -49,14 +96,14 @@ Section __.
       let/n Z2:= (AA+Z2) in
       let/n Z2 := E*Z2 in
       (* ((X4, Z4), (X5, Z5)) *)
-      ((X2, Z2), (X3, Z3)).
+      ret ((X2, Z2), (X3, Z3)).
   End Gallina.
 
   Instance spec_of_ladderstep : spec_of "ladderstep" :=
     fnspec! "ladderstep"
           (pX1 pX2 pZ2 pX3 pZ3
-               pA pAA pB pBB pE pC pD pDA pCB : word)
-          / (X1 X2 Z2 X3 Z3 A AA B BB E C D DA CB : felem) R,
+               (*pA pAA pB pBB pE pC pD pDA pCB*) : Semantics.word)
+          / (X1 X2 Z2 X3 Z3 (*A AA B BB E C D DA CB*) : felem) R,
     { requires tr mem :=
         bounded_by tight_bounds X1
         /\ bounded_by tight_bounds X2
@@ -66,43 +113,46 @@ Section __.
         /\ (FElem pX1 X1
             * FElem pX2 X2 * FElem pZ2 Z2
             * FElem pX3 X3 * FElem pZ3 Z3
-            * FElem pA A * FElem pAA AA
+            (** FElem pA A * FElem pAA AA
             * FElem pB B * FElem pBB BB
             * FElem pE E * FElem pC C
             * FElem pD D * FElem pDA DA
-            * FElem pCB CB * R)%sep mem;
-      ensures tr' mem' :=
-        tr = tr'
-        /\ exists X4 Z4 X5 Z5 (* output values *)
-               A' AA' B' BB' E' C' D' DA' CB' (* new intermediates *)
-               : felem,
-          (ladderstep_gallina
-             (feval X1) (feval X2, feval Z2)
-             (feval X3, feval Z3)
-           = ((feval X4, feval Z4), (feval X5, feval Z5)))
-          /\ bounded_by tight_bounds X4
-          /\ bounded_by tight_bounds Z4
-          /\ bounded_by tight_bounds X5
-          /\ bounded_by tight_bounds Z5
-          /\ (FElem pX1 X1 * FElem pX2 X4 * FElem pZ2 Z4
-              * FElem pX3 X5 * FElem pZ3 Z5
-              * FElem pA A' * FElem pAA AA'
-              * FElem pB B' * FElem pBB BB'
-              * FElem pE E' * FElem pC C' * FElem pD D'
-              * FElem pDA DA' * FElem pCB CB' * R)%sep mem'}.
+            * FElem pCB CB*) * R)%sep mem;
+      ensures tr' mem' rets :=
+        (propbind
+           (ladderstep_gallina
+              (feval X1) (feval X2, feval Z2)
+              (feval X3, feval Z3))
+           (fun res =>
+              rets = [] /\
+             tr = tr'
+             /\ exists X4 Z4 X5 Z5 (* output values *)
+                       (*A' AA' B' BB' E' C' D' DA' CB' (* new intermediates *)*)
+                       : felem,
+               (res = ((feval X4, feval Z4), (feval X5, feval Z5)))
+        /\ bounded_by tight_bounds X4
+        /\ bounded_by tight_bounds Z4
+        /\ bounded_by tight_bounds X5
+        /\ bounded_by tight_bounds Z5
+        /\ (FElem pX1 X1 * FElem pX2 X4 * FElem pZ2 Z4
+            * FElem pX3 X5 * FElem pZ3 Z5
+            (** FElem pA A' * FElem pAA AA'
+             * FElem pB B' * FElem pBB BB'
+             * FElem pE E' * FElem pC C' * FElem pD D'
+             * FElem pDA DA' * FElem pCB CB'*) * R)%sep mem'))}.
 
   Lemma compile_ladderstep : forall {tr mem locals functions}
         (x1 x2 z2 x3 z3 : F M_pos),
     let v := ladderstep_gallina x1 (x2, z2) (x3, z3) in
-    forall {P} {pred: P v -> predicate} {k: nlet_eq_k P v} {k_impl}
+    forall {P} {pred: P -> predicate} {k: (point *point) -> Comp P} {k_impl}
            Rout
            X1 X1_ptr X1_var X2 X2_ptr X2_var Z2 Z2_ptr Z2_var
            X3 X3_ptr X3_var Z3 Z3_ptr Z3_var
-           A A_ptr A_var AA AA_ptr AA_var
+          (* A A_ptr A_var AA AA_ptr AA_var
            B B_ptr B_var BB BB_ptr BB_var
            E E_ptr E_var C C_ptr C_var
            D D_ptr D_var DA DA_ptr DA_var
-           CB CB_ptr CB_var,
+           CB CB_ptr CB_var*),
 
       spec_of_ladderstep functions ->
 
@@ -119,18 +169,18 @@ Section __.
       (FElem X1_ptr X1
        * FElem X2_ptr X2 * FElem Z2_ptr Z2
        * FElem X3_ptr X3 * FElem Z3_ptr Z3
-       * FElem A_ptr A * FElem AA_ptr AA
+      (* * FElem A_ptr A * FElem AA_ptr AA
        * FElem B_ptr B * FElem BB_ptr BB
        * FElem E_ptr E * FElem C_ptr C
        * FElem D_ptr D * FElem DA_ptr DA
-       * FElem CB_ptr CB * Rout)%sep mem ->
+       * FElem CB_ptr CB *) * Rout)%sep mem ->
 
         map.get locals X1_var = Some X1_ptr ->
         map.get locals X2_var = Some X2_ptr ->
         map.get locals Z2_var = Some Z2_ptr ->
         map.get locals X3_var = Some X3_ptr ->
         map.get locals Z3_var = Some Z3_ptr ->
-        map.get locals A_var = Some A_ptr ->
+        (*map.get locals A_var = Some A_ptr ->
         map.get locals AA_var = Some AA_ptr ->
         map.get locals B_var = Some B_ptr ->
         map.get locals BB_var = Some BB_ptr ->
@@ -138,32 +188,35 @@ Section __.
         map.get locals C_var = Some C_ptr ->
         map.get locals D_var = Some D_ptr ->
         map.get locals DA_var = Some DA_ptr ->
-        map.get locals CB_var = Some CB_ptr ->
+        map.get locals CB_var = Some CB_ptr ->*)
 
         (let v := v in
          forall (X4 Z4 X5 Z5 (* output values *)
-                    A' AA' B' BB' E' C' D' DA' CB' (* new intermediates *)
+                    (*A' AA' B' BB' E' C' D' DA' CB' (* new intermediates *)*)
                  : felem) m
-                (Heq : ladderstep_gallina
-                         (feval X1) (feval X2, feval Z2)
-                         (feval X3, feval Z3)
-                       = ((feval X4, feval Z4), (feval X5, feval Z5))),
+                (Heq : propbind
+                         (ladderstep_gallina
+                            (feval X1) (feval X2, feval Z2)
+                            (feval X3, feval Z3))
+                         (eq ((feval X4, feval Z4), (feval X5, feval Z5)))),
           bounded_by tight_bounds X4 ->
           bounded_by tight_bounds Z4 ->
           bounded_by tight_bounds X5 ->
           bounded_by tight_bounds Z5 ->
           (FElem X1_ptr X1 * FElem X2_ptr X4 * FElem Z2_ptr Z4
            * FElem X3_ptr X5 * FElem Z3_ptr Z5
-           * FElem A_ptr A' * FElem AA_ptr AA'
+           (* * FElem A_ptr A' * FElem AA_ptr AA'
            * FElem B_ptr B' * FElem BB_ptr BB'
            * FElem E_ptr E' * FElem C_ptr C' * FElem D_ptr D'
-           * FElem DA_ptr DA' * FElem CB_ptr CB' * Rout)%sep m ->
+           * FElem DA_ptr DA' * FElem CB_ptr CB' *) * Rout)%sep m ->
            (<{ Trace := tr;
                Memory := m;
                Locals := locals;
                Functions := functions }>
             k_impl
-            <{ pred (k v eq_refl) }>)) ->
+            <{ pbind pred (bindn
+                   [X1_var; X2_var; Z2_var; X3_var; Z3_var]
+                   v k) }>)) ->
 
         <{ Trace := tr;
            Memory := mem;
@@ -173,22 +226,46 @@ Section __.
           (cmd.call [] "ladderstep"
                     [ expr.var X1_var; expr.var X2_var;
                         expr.var Z2_var; expr.var X3_var;
-                          expr.var Z3_var; expr.var A_var;
+                          expr.var Z3_var (*; expr.var A_var;
                             expr.var AA_var; expr.var B_var;
                               expr.var BB_var; expr.var E_var;
                                 expr.var C_var; expr.var D_var;
-                                  expr.var DA_var; expr.var CB_var ])
+                                  expr.var DA_var; expr.var CB_var *)])
           k_impl
-        <{ pred (nlet_eq
+        <{ pbind pred (bindn
                    [X1_var; X2_var; Z2_var; X3_var; Z3_var]
                    v k) }>.
     Proof.
       repeat straightline'.
-      handle_call;
+      handle_call. 
         lazymatch goal with
         | |- sep _ _ _ => ecancel_assumption
         | _ => solve [eauto]
         end.
+        lazymatch goal with
+        | |- sep _ _ _ => ecancel_assumption
+        | _ => solve [eauto]
+        end.
+        lazymatch goal with
+        | |- sep _ _ _ => ecancel_assumption
+        | _ => solve [eauto]
+        end.
+        lazymatch goal with
+        | |- sep _ _ _ => ecancel_assumption
+        | _ => solve [eauto]
+        end.
+        lazymatch goal with
+        | |- sep _ _ _ => ecancel_assumption
+        | _ => solve [eauto]
+        end.
+        destruct H17.
+        unfold intersection in H17.
+        repeat straightline.
+        eapply H16.
+        6:eauto.
+        all: eauto.
+        exists x.
+        split; eauto.
     Qed.
 
   Ltac ladderstep_compile_custom :=
@@ -202,13 +279,46 @@ Section __.
            end.
 
   Ltac compile_custom ::= ladderstep_compile_custom.
+  
+  Hint Extern 1 => simple eapply compile_stack_alloc; shelve : compiler.
+  
+  Hint Unfold pbind: compiler_cleanup.
+  Hint Extern 1 (ret _ _) => reflexivity : compiler_cleanup.
+  Hint Resolve compile_setup_nondet_pbind : compiler_setup.
+  Hint Extern 2 (IsRupicolaBinding (bindn _ _ _)) => exact true : typeclass_instances.
+  
+Definition
+  ladderstep_body' :=
+  noskips
+  (cmd.seq (cmd.call [] add [expr.var "X2"; expr.var "Z2"; expr.var "A"])
+     (cmd.seq (cmd.call [] square [expr.var "A"; expr.var "AA"])
+        (cmd.seq (cmd.call [] sub [expr.var "X2"; expr.var "Z2"; expr.var "B"])
+           (cmd.seq (cmd.call [] square [expr.var "B"; expr.var "BB"])
+              (cmd.seq (cmd.call [] sub [expr.var "AA"; expr.var "BB"; expr.var "E"])
+                 (cmd.seq (cmd.call [] add [expr.var "X3"; expr.var "Z3"; expr.var "C"])
+                    (cmd.seq (cmd.call [] sub [expr.var "X3"; expr.var "Z3"; expr.var "D"])
+                       (cmd.seq (cmd.call [] mul [expr.var "D"; expr.var "A"; expr.var "DA"])
+                          (cmd.seq (cmd.call [] mul [expr.var "C"; expr.var "B"; expr.var "CB"])
+                             (cmd.seq (cmd.call [] add [expr.var "DA"; expr.var "CB"; expr.var "X3"])
+                                (cmd.seq (cmd.call [] square [expr.var "X3"; expr.var "X3"])
+                                   (cmd.seq (cmd.call [] sub [expr.var "DA"; expr.var "CB"; expr.var "Z3"])
+                                      (cmd.seq (cmd.call [] square [expr.var "Z3"; expr.var "Z3"])
+                                         (cmd.seq (cmd.call [] mul [expr.var "X1"; expr.var "Z3"; expr.var "Z3"])
+                                            (cmd.seq
+                                               (cmd.call [] mul [expr.var "AA"; expr.var "BB"; expr.var "X2"])
+                                               (cmd.seq (cmd.call [] scmula24 [expr.var "E"; expr.var "Z2"])
+                                                  (cmd.seq
+                                                     (cmd.call [] add
+                                                        [expr.var "AA"; expr.var "Z2"; expr.var "Z2"])
+                                                     (cmd.seq
+                                                        (cmd.call [] mul
+                                                           [expr.var "E"; expr.var "Z2"; expr.var "Z2"])
+                                                        (fold_right
+                                                           (fun (v : string) (c : cmd) => cmd.seq (cmd.unset v) c)
+                                                           cmd.skip []))))))))))))))))))).
 
-  Hint Extern 1 (spec_of _) => (simple refine (@spec_of_BinOp _ _ _ _ _ _ _ _ _ _)) : typeclass_instances.
-  Hint Extern 1 (spec_of _) => (simple refine (@spec_of_UnOp _ _ _ _ _ _ _ _ _ _)) : typeclass_instances.
-  Derive ladderstep_body SuchThat
-         (let args := ["X1"; "X2"; "Z2"; "X3"; "Z3";
-                         "A"; "AA"; "B"; "BB"; "E"; "C";
-                         "D"; "DA"; "CB"] in
+Derive ladderstep_body SuchThat
+         (let args := ["X1"; "X2"; "Z2"; "X3"; "Z3"] in
           ltac:(
             let proc := constr:(("ladderstep",
                                  (args, [], ladderstep_body))
@@ -218,10 +328,10 @@ Section __.
             exact (__rupicola_program_marker ladderstep_gallina -> goal)))
          As ladderstep_correct.
   Proof.
-    compile_setup.
-
-    repeat compile_step.
+    compile.
   Qed.
+
+  
 End __.
 
 Existing Instance spec_of_ladderstep.
